implement iarray_vec4_read_cells

src/lib/data/Kuiper.Vectorized.fsti
@@ -2,28 +2,12 @@ module Kuiper.Vectorized
 
 #lang-pulse
 
-// open Pulse.Lib.Vec
-// open Pulse
-// open Pulse.Lib.BigStar
-module T = FStar.Tactics.V2
 open FStar.Seq
 
 open Kuiper
 open Kuiper.IView
-open Kuiper.IArray
-// open Kuiper.Array
-// open Kuiper.Base
-// open Kuiper.Sized
-// open Kuiper.SizeT
-// open Kuiper.Seq.Common
 
 module SZ = FStar.SizeT
-
-// class has_vec_t (et : Type0) = {
-//   vec_lens : seq nat;
-//   vec_ts : seq Type0;
-//   _eq_len : squash (length vec_lens == length vec_ts)
-// }
 
 new
 val float4 : Type0
@@ -66,18 +50,6 @@ val lemma_getw_projects_w (x : float) (y : float) (z : float) (w : float)
 new
 val lemma_make_float4_from_float4 (v : float4)
   : Lemma (ensures make_float4 (getx v) (gety v) (getz v) (getw v) == v)
-
-// let vec_t (et : Type0) (vec_sz : erased nat)
-//   = match (et, reveal vec_sz) with
-//     // | (f32, 1) -> Some(vf32_1)
-//     // | (f32, 2) -> Some(vf32_2)
-//     // | (f32, 3) -> Some(vf32_3)
-//     | (f32, 4) -> Some(vf32_4)
-//     // | (f64, 1) -> Some(vf32_1)
-//     // | (f64, 2) -> Some(vf32_2)
-//     // | (f64, 3) -> Some(vf32_3)
-//     // | (f64, 4) -> Some(v4_64)
-//     | _ -> None
 
 [@@noextract_to "krml"]
 atomic
@@ -133,56 +105,3 @@ fn gpu_array_write_vec4
                 i <= SZ.v idx /\ SZ.v idx + 3 < j /\
                 s' == upd_seq_vec4 s (idx - i) v))
 
-open Kuiper.Injection
-
-let ai_add
-  (#len : nat)
-  (vw : aiview len)
-  (ai : vw.sch.ait)
-  (x : nat{in_image vw.step.imap.f ((it_to_nat vw ai) + x)})
-  : GTot vw.sch.ait  = ((it_to_nat vw ai) + x) <~| vw.step.imap
-
-let iarray_pts_to_4cells
-  (#et:Type0)
-  (#len : erased nat) (#vw : aiview len)
-  ([@@@mkey] a : iarray et vw)
-  (#[T.exact (`1.0R)] f : perm)
-  ([@@@mkey] ai : vw.sch.ait)
-  // Should probably be restricted to only the elements that are accessed?
-  //  this: (#v : (ai: vw.sch.ait{0 <= vw.sch.bij.ff ai /\ vw.sch.bij.ff ai < 4} -> GTot float))
-  (v : (vw.sch.ait -> GTot et))
-  (_ : squash (forall (x : natlt 4). in_image vw.step.imap.f ((it_to_nat vw ai) + x)))
-  : slprop
-  =
-  // pure (SZ.fits len) **
-    iarray_pts_to_cell a #f ai (v ai) ** 
-    iarray_pts_to_cell a #f (ai_add vw ai 1) (v ai) ** 
-    iarray_pts_to_cell a #f (ai_add vw ai 2) (v ai) ** 
-    iarray_pts_to_cell a #f (ai_add vw ai 3) (v ai)
-
-#push-options "--debug SMTFail --split_queries always"
-fn iarray_vec4_read_cells
-  // (#et:Type0)
-  (#len : erased nat)
-  (#vw : aiview len) {| cw : ciview vw |}
-  // (a : iarray et vw)
-  (a : iarray float vw)
-  (ci : cw.sch.cit{vw.sch.ait_enum.bij.ff (cw.sch.bij.gg ci) + 3 < vw.sch.ait_enum._cardinal})
-  (#f : perm)
-  // Should probably be restricted to only the elements that are accessed?
-  //  this: (#v : (ai: vw.sch.ait{0 <= vw.sch.bij.ff ai /\ vw.sch.bij.ff ai < 4} -> GTot float))
-  (#v : (vw.sch.ait -> GTot float))
-  (_ : squash (forall (x : natlt 4). in_image vw.step.imap.f (it_to_nat vw (ci_to_ai vw ci) + x)))
-  preserves gpu
-  preserves iarray_pts_to_4cells #float a #f (ci_to_ai vw ci) v
-  returns
-    e : float4
-  ensures
-    pure (e == make_float4
-                 (v (ci_to_ai vw ci))
-                 (v (ai_add vw (ci_to_ai vw ci)  1))
-                 (v (ai_add vw (ci_to_ai vw ci)  2))
-                 (v (ai_add vw (ci_to_ai vw ci)  3)))
-{
-  admit();
-}
