src/lib/data/Kuiper.Vectorized.IArray.fst
@@ -1,0 +1,130 @@
+module Kuiper.Vectorized.IArray
+
+#lang-pulse
+
+module T = FStar.Tactics.V2
+open FStar.Seq
+
+open Kuiper
+open Kuiper.IView
+open Kuiper.Vectorized
+
+friend Kuiper.IArray
+open Kuiper.IArray
+
+module SZ = FStar.SizeT
+
+open Kuiper.Injection
+
+let ai_add
+  (#len : nat)
+  (vw : aiview len)
+  (ai : vw.sch.ait)
+  (x : nat{in_image vw.step.imap.f ((it_to_nat vw ai) + x)})
+  : GTot vw.sch.ait  = it_of_nat vw ((it_to_nat vw ai) + x)
+
+let iarray_pts_to_4cells
+  (#et:Type0)
+  (#len : erased nat) (#vw : aiview len)
+  ([@@@mkey] a : iarray et vw)
+  (#[T.exact (`1.0R)] f : perm)
+  ([@@@mkey] ai : vw.sch.ait)
+  // Should probably be restricted to only the elements that are accessed?
+  //  this: (#v : (ai: vw.sch.ait{0 <= vw.sch.bij.ff ai /\ vw.sch.bij.ff ai < 4} -> GTot float))
+  (v : et & et & et & et)
+  : slprop
+  =
+    Pulse.Lib.WithPure.with_pure
+      ((forall (x : natlt 4). in_image vw.step.imap.f ((it_to_nat vw ai) + x)))
+      (fun _ ->
+        // pure (SZ.fits len) **
+          iarray_pts_to_cell a #f ai               v._1 ** 
+          iarray_pts_to_cell a #f (ai_add vw ai 1) v._2 ** 
+          iarray_pts_to_cell a #f (ai_add vw ai 2) v._3 ** 
+          iarray_pts_to_cell a #f (ai_add vw ai 3) v._4)
+
+// #push-options "--debug SMTFail --split_queries always"
+// #push-options "--print-implicits"
+fn iarray_vec4_read_cells
+  // (#et:Type0)
+  (#len : erased nat)
+  (#vw : aiview len) {| cw : ciview vw |}
+  // (a : iarray et vw)
+  (a : iarray float vw)
+  (ci : cw.sch.cit)
+  (#f : perm)
+  // Should probably be restricted to only the elements that are accessed?
+  //  this: (#v : (ai: vw.sch.ait{0 <= vw.sch.bij.ff ai /\ vw.sch.bij.ff ai < 4} -> GTot float))
+  (v : erased (float & float & float & float))
+  // (_ : squash (forall (x : natlt 4). in_image vw.step.imap.f (it_to_nat vw (ci_to_ai vw ci) + x)))
+  preserves gpu
+  preserves iarray_pts_to_4cells #float a #f (ci_to_ai vw ci) v
+  returns
+    e : float4
+  ensures
+    pure (e == make_float4 (reveal v)._1 (reveal v)._2 (reveal v)._3 (reveal v)._4)
+{
+  (* get gpu_pts_to_slice *)
+  unfold iarray_pts_to_4cells a #f (ci_to_ai vw ci) v;
+
+  unfold iarray_pts_to_cell a #f (ci_to_ai vw ci) (reveal v)._1;
+  unfold iarray_pts_to_cell a #f (ai_add vw (ci_to_ai vw ci) 1) (reveal v)._2;
+  unfold iarray_pts_to_cell a #f (ai_add vw (ci_to_ai vw ci) 2) (reveal v)._3;
+  unfold iarray_pts_to_cell a #f (ai_add vw (ci_to_ai vw ci) 3) (reveal v)._4;
+
+  (* make index look the same for concatenation *)
+  rewrite each gpu_pts_to_slice (core a) #f (ci_to_ai vw ci |~> vw.step.imap) ((ci_to_ai vw ci |~> vw.step.imap) + 1)  seq![(reveal v)._1]
+  as gpu_pts_to_slice (core a) #f (ai_add vw (ci_to_ai vw ci) 0 |~> vw.step.imap) ((ai_add vw (ci_to_ai vw ci) 0 |~> vw.step.imap) + 1) seq![(reveal v)._1];
+
+  rewrite each ((ai_add vw (ci_to_ai vw ci) 0 |~> vw.step.imap) + 1) as ((ai_add vw (ci_to_ai vw ci) 1 |~> vw.step.imap));
+  rewrite each ((ai_add vw (ci_to_ai vw ci) 1 |~> vw.step.imap) + 1) as ((ai_add vw (ci_to_ai vw ci) 2 |~> vw.step.imap));
+  rewrite each ((ai_add vw (ci_to_ai vw ci) 2 |~> vw.step.imap) + 1) as ((ai_add vw (ci_to_ai vw ci) 3 |~> vw.step.imap));
+
+  (* concatenate into a single slice *)
+  gpu_slice_concat (core a) #f
+    (ai_add vw (ci_to_ai vw ci) 0 |~> vw.step.imap)
+    (ai_add vw (ci_to_ai vw ci) 1 |~> vw.step.imap)
+    ((ai_add vw (ci_to_ai vw ci) 1 |~> vw.step.imap) + 1);
+  gpu_slice_concat (core a) #f
+    (ai_add vw (ci_to_ai vw ci) 0 |~> vw.step.imap)
+    (ai_add vw (ci_to_ai vw ci) 2 |~> vw.step.imap)
+    ((ai_add vw (ci_to_ai vw ci) 2 |~> vw.step.imap) + 1);
+   gpu_slice_concat (core a) #f
+    (ai_add vw (ci_to_ai vw ci) 0 |~> vw.step.imap)
+    (ai_add vw (ci_to_ai vw ci) 3 |~> vw.step.imap)
+    ((ai_add vw (ci_to_ai vw ci) 3 |~> vw.step.imap) + 1);
+
+  (* read from array *)
+  cw.step.compat (ci |> cw.sch.bij.gg);
+  let flat_idx = ci |~> cw.step.cimap;
+  let v' = gpu_array_read_vec4 (core a) flat_idx;
+
+  (* split full slice back into multiple *)
+  gpu_slice_split (core a) #f
+    (ai_add vw (ci_to_ai vw ci) 0 |~> vw.step.imap)
+    (ai_add vw (ci_to_ai vw ci) 3 |~> vw.step.imap)
+    ((ai_add vw (ci_to_ai vw ci) 3 |~> vw.step.imap) + 1);
+  gpu_slice_split (core a) #f
+    (ai_add vw (ci_to_ai vw ci) 0 |~> vw.step.imap)
+    (ai_add vw (ci_to_ai vw ci) 2 |~> vw.step.imap)
+    ((ai_add vw (ci_to_ai vw ci) 2 |~> vw.step.imap) + 1);
+  gpu_slice_split (core a) #f
+    (ai_add vw (ci_to_ai vw ci) 0 |~> vw.step.imap)
+    (ai_add vw (ci_to_ai vw ci) 1 |~> vw.step.imap)
+    ((ai_add vw (ci_to_ai vw ci) 1 |~> vw.step.imap) + 1);
+
+  (* reverse how index looks *)
+  rewrite each gpu_pts_to_slice (core a) #f (ai_add vw (ci_to_ai vw ci) 0 |~> vw.step.imap) (ai_add vw (ci_to_ai vw ci) 1 |~> vw.step.imap) seq![(reveal v)._1]
+  as gpu_pts_to_slice (core a) #f (ci_to_ai vw ci |~> vw.step.imap) ((ci_to_ai vw ci |~> vw.step.imap) + 1)  seq![(reveal v)._1];
+
+  (* fold back *)
+  fold iarray_pts_to_cell a #f (ci_to_ai vw ci) (reveal v)._1;
+  fold iarray_pts_to_cell a #f (ai_add vw (ci_to_ai vw ci) 1) (reveal v)._2;
+  fold iarray_pts_to_cell a #f (ai_add vw (ci_to_ai vw ci) 2) (reveal v)._3;
+  fold iarray_pts_to_cell a #f (ai_add vw (ci_to_ai vw ci) 3) (reveal v)._4;
+
+  fold iarray_pts_to_4cells a #f (ci_to_ai vw ci) v;
+  
+  (* return float4 *)
+  v'
+}
