src/lib/data/Kuiper.Vectorized.IArray.fsti
@@ -1,0 +1,1 @@
+module Kuiper.Vectorized.IArray
